reorganize Interpolation files

Pdl/InterpolationDef.lean
@@ -1,466 +1,13 @@
 import Pdl.Flip
+import Pdl.LocalInterpolation
 import Pdl.Soundness
 
-/-! # Interpolants for Partitions (Section 9)
+/-! # Defining interpolants (Section 9)
 
-Note that we can skip much of subsection 8.2 because we worked already with split tableaux anyway.
+Note that we can skip much of Subsection 8.2 because we worked already with split tableaux anyway.
 
 NOTE: We may need extra work for *uniformity* though.
 -/
-
-open HasSat
-
-/-! ## Joint vocabulary -/
-
-/-- The joint vocabulary occurring on both the left and the right side. -/
-@[simp]
-def jvoc (X : Sequent) : Vocab := (X.left).fvoc ∩ (X.right).fvoc
-
-lemma jvoc_sub_of_voc_sub {Y X : Sequent}
-    (hl : Y.left.fvoc ⊆ X.left.fvoc)
-    (hr : Y.right.fvoc ⊆ X.right.fvoc)
-    : jvoc Y ⊆ jvoc X := by
-  intro x x_in_jY
-  simp only [jvoc, Finset.mem_inter] at x_in_jY
-  specialize @hl x x_in_jY.1
-  specialize @hr x x_in_jY.2
-  simp only [jvoc, Finset.mem_inter]
-  tauto
-
-/-! ## Partition Interpolants -/
-
-def isPartInterpolant (X : Sequent) (θ : Formula) :=
-  θ.voc ⊆ jvoc X ∧ (¬ satisfiable ((~θ) :: X.left) ∧ ¬ satisfiable (θ :: X.right))
-
-def PartInterpolant (N : Sequent) := Subtype <| isPartInterpolant N
-
-/-- Like `Olf.voc` but without the ⊕ inside. -/
-def onlfvoc : Option NegLoadFormula → Vocab
-| none => ∅
-| some nlf => NegLoadFormula.voc nlf
-
-def lfovoc (L : List (List Formula × Option NegLoadFormula)) : Vocab :=
-  L.toFinset.sup (fun ⟨fs,o⟩ => fs.fvoc ∪ (onlfvoc o))
-
-/-! ## Interpolants for local rules -/
-
-lemma LoadRule_voc (lr : LoadRule (~'χ) ress) : lfovoc ress ⊆ χ.voc := by
-  intro x x_in
-  unfold lfovoc at x_in
-  simp at x_in
-  rcases x_in with ⟨fs, onlf, in_ress, x_in_V⟩
-  cases lr
-  case dia α χ notAtom =>
-    have unfvoc := @unfoldDiamond_voc x α χ.unload
-    rw [← unfoldDiamondLoaded_eq α χ] at unfvoc
-    specialize @unfvoc (pairUnload (fs, onlf)) (by simp only [List.mem_map]; use (fs,onlf))
-    rcases onlf with _ | ⟨⟨lf⟩⟩  <;> simp [onlfvoc] at *
-    · rcases x_in_V with ⟨f, f_in_fs, x_in⟩
-      specialize unfvoc f_in_fs
-      aesop
-    · simp [pairUnload] at unfvoc
-      rcases x_in_V with ⟨f, f_in_fs, x_in⟩|_ <;> aesop
-  case dia' α φ notAtom =>
-    have unfvoc := @unfoldDiamond_voc x α φ
-    rw [← unfoldDiamondLoaded'_eq α φ] at unfvoc
-    specialize @unfvoc (pairUnload (fs, onlf)) (by simp only [List.mem_map]; use (fs,onlf))
-    rcases onlf with _ | ⟨⟨lf⟩⟩  <;> simp [onlfvoc] at *
-    · rcases x_in_V with ⟨f, f_in_fs, x_in⟩
-      specialize unfvoc f_in_fs
-      aesop
-    · simp [pairUnload] at unfvoc
-      rcases x_in_V with ⟨f, f_in_fs, x_in⟩|_ <;> aesop
-
-theorem localRule_does_not_increase_vocab_L {Cond B}
-    (rule : LocalRule Cond B) :
-    ∀ res ∈ B, res.left.fvoc ⊆ Cond.left.fvoc := by
-  rcases Cond with ⟨Lcond, Rcond, Ocond⟩
-  intro res res_in_B x x_in_res
-  cases rule
-  case oneSidedL ress orule B_def =>
-    subst B_def
-    simp at res_in_B
-    rcases res_in_B with ⟨L, L_in, def_res⟩
-    subst def_res
-    simp at *
-    rcases x_in_res with ⟨ψ, ψ_in, x_in_voc_ψ⟩
-    cases orule
-    case nCo => aesop
-    case box α φ α_notAt => have := unfoldBox_voc L_in ψ_in x_in_voc_ψ; simp_all
-    case dia => have := unfoldDiamond_voc L_in ψ_in x_in_voc_ψ; simp_all
-    all_goals aesop
-  case loadedL ress χ lrule B_def =>
-    subst B_def
-    simp at res_in_B
-    rcases res_in_B with ⟨L, lnf, in_ress, def_res⟩
-    subst def_res
-    simp only [List.fvoc, Vocab.fromList, Sequent.left, Sequent.L, Sequent.O, List.map_append,
-      List.toFinset_append, Finset.mem_sup, Finset.mem_union, List.mem_toFinset, List.mem_map,
-      id_eq, List.empty_eq, List.nil_append, exists_exists_and_eq_and] at *
-    rcases x_in_res with ⟨φvoc, ⟨φ, φ_in_L, def_φvoc⟩|⟨φ, φ_in_OlfL, def_φvoc⟩, x_in_φvoc⟩
-    all_goals
-      subst def_φvoc
-      simp only [Olf.L, List.mem_cons, List.not_mem_nil, or_false, exists_eq_left, Formula.voc]
-      have := LoadRule_voc lrule
-      simp only [lfovoc, List.fvoc, Vocab.fromList, LoadFormula.voc] at this
-      apply this; clear this
-      simp [onlfvoc]
-      refine ⟨L, lnf, in_ress, ?_⟩
-    · left
-      use φ
-    · right
-      cases lnf <;> simp [Olf.L] at *
-      subst φ_in_OlfL
-      exact x_in_φvoc
-  -- other cases are all trivial (as in Bml)
-  all_goals
-    aesop
-
-theorem localRule_does_not_increase_vocab_R (rule : LocalRule Cond B) :
-    ∀ res ∈ B, res.right.fvoc ⊆ Cond.right.fvoc := by
-  rcases Cond with ⟨Lcond, Rcond, Ocond⟩
-  intro res res_in_B x x_in_res
-  cases rule
-  case oneSidedR ress orule B_def =>
-    subst B_def
-    simp at res_in_B
-    rcases res_in_B with ⟨L, L_in, def_res⟩
-    subst def_res
-    simp at *
-    rcases x_in_res with ⟨ψ, ψ_in, x_in_voc_ψ⟩
-    cases orule
-    case nCo => aesop
-    case box α φ α_notAt => have := unfoldBox_voc L_in ψ_in x_in_voc_ψ; simp_all
-    case dia => have := unfoldDiamond_voc L_in ψ_in x_in_voc_ψ; simp_all
-    all_goals aesop
-  case loadedR ress χ lrule B_def =>
-    subst B_def
-    simp at res_in_B
-    rcases res_in_B with ⟨L, lnf, in_ress, def_res⟩
-    subst def_res
-    simp only [List.fvoc, Vocab.fromList, Sequent.right, Sequent.R, Sequent.O, List.map_append,
-      List.toFinset_append, Finset.mem_sup, Finset.mem_union, List.mem_toFinset, List.mem_map,
-      id_eq, List.empty_eq, List.nil_append, exists_exists_and_eq_and] at *
-    rcases x_in_res with ⟨φvoc, ⟨φ, φ_in_L, def_φvoc⟩|⟨φ, φ_in_OlfR, def_φvoc⟩, x_in_φvoc⟩
-    all_goals
-      subst def_φvoc
-      simp only [Olf.R, List.mem_cons, List.not_mem_nil, or_false, exists_eq_left, Formula.voc]
-      have := LoadRule_voc lrule
-      simp only [lfovoc, List.fvoc, Vocab.fromList, LoadFormula.voc] at this
-      apply this; clear this
-      simp [onlfvoc]
-      refine ⟨L, lnf, in_ress, ?_⟩
-    · left
-      use φ
-    · right
-      cases lnf <;> simp [Olf.R] at *
-      subst φ_in_OlfR
-      exact x_in_φvoc
-  -- other cases are all trivial (as in Bml)
-  all_goals
-    aesop
-
-theorem localRuleApp_does_not_increase_jvoc (lra : LocalRuleApp) :
-    ∀ Y ∈ lra.C, jvoc Y ⊆ jvoc lra.X := by
-  match lra with
-  | @LocalRuleApp.mk L R O Lcond Rcond Ocond ress lrule C hC preconditionProof =>
-    subst hC
-    rintro ⟨cL, cR, cO⟩ C_in
-    simp [applyLocalRule] at C_in
-    rcases C_in with ⟨⟨Lres, Rres, Ores⟩ , res_in, cLRO_def⟩
-    simp at cLRO_def
-    cases cLRO_def
-    apply jvoc_sub_of_voc_sub -- hhmmm?
-    · intro x x_in
-      simp at * -- only
-      rcases x_in with ⟨φvoc, ⟨φ, φ_nocon, d_φvoc⟩|⟨φ, φ_L, d_φvoc⟩|⟨φ, φ_O, d_φvoc⟩, x_in_φvoc⟩
-      all_goals subst d_φvoc
-      · refine ⟨φ.voc, Or.inl ?_, x_in_φvoc⟩
-        exact ⟨φ, List.diff_subset L Lcond φ_nocon, rfl⟩
-      all_goals
-        have Lsub := @localRule_does_not_increase_vocab_L _ _ lrule _ res_in x
-        simp at Lsub
-      · specialize Lsub φ.voc (Or.inl ⟨_, φ_L, rfl⟩) x_in_φvoc
-        rcases Lsub with ⟨ψvoc, h_ψvoc, x_in_ψvoc⟩
-        refine ⟨ψvoc, ?_, x_in_ψvoc⟩
-        rcases h_ψvoc with (⟨ψ, ψ_in_Lcond, d_ψvoc⟩ | ⟨ψ, ψ_in_Ocond, d_ψvoc⟩) <;> subst d_ψvoc
-        · exact Or.inl ⟨ψ, preconditionProof.1.subset ψ_in_Lcond, rfl⟩
-        · refine Or.inr ⟨ψ, ?_, rfl⟩; aesop
-      · -- whether to use φ.voc depends on whether the localRuleApp changes the O here.
-        rcases O with _|χ <;> rcases Ocond with _|cχ <;> rcases Ores with _|resχ
-        all_goals
-          simp [Olf.change] at * -- already treats 3 cases
-        · specialize Lsub φ.voc (Or.inr ⟨φ, φ_O, rfl⟩) x_in_φvoc
-          rcases Lsub with ⟨ψ, ψ_in_Lcond, x_in_φvoc⟩
-          exact ⟨ψ, preconditionProof.1.subset ψ_in_Lcond, x_in_φvoc⟩
-        · rcases χ with ⟨⟨χ⟩⟩|⟨χ⟩ <;> simp [Olf.L] at *
-          subst φ_O
-          aesop
-        · rcases resχ with ⟨⟨resχ⟩⟩|⟨⟨resχ⟩⟩ <;> simp [Olf.L] at φ_O Lsub
-          subst φ_O
-          simp at x_in_φvoc
-          specialize Lsub (resχ.unload).voc (Or.inr rfl) x_in_φvoc
-          rcases Lsub with ⟨ψ, ψ_in_Lcond, x_in_φvoc⟩
-          exact ⟨ψ.voc, Or.inl ⟨ψ, preconditionProof.1.subset ψ_in_Lcond, rfl⟩, x_in_φvoc⟩
-        · rcases preconditionProof with ⟨Lin, Rin, same_form⟩
-          subst same_form
-          simp at φ_O
-        · specialize Lsub φ.voc (Or.inr ⟨φ, φ_O, rfl⟩) x_in_φvoc
-          rcases Lsub with ⟨ψvoc, ψ_defs, x_in_ψvoc⟩
-          rcases ψ_defs with ⟨ψ, ψ_in, ψvoc_def⟩|⟨ψ, ψ_in, ψvoc_def⟩ <;> subst ψvoc_def
-          · exact ⟨ψ.voc, Or.inl ⟨ψ, preconditionProof.1.subset ψ_in, rfl⟩, x_in_ψvoc⟩
-          · refine ⟨ψ.voc, Or.inr ⟨ψ, ?_, rfl⟩, x_in_ψvoc⟩
-            simp_all
-    · -- analogous to L side, but quite some modifications
-      intro x x_in
-      simp at * -- only
-      rcases x_in with ⟨φvoc, ⟨φ, φ_nocon, d_φvoc⟩|⟨φ, φ_L, d_φvoc⟩|⟨φ, φ_O, d_φvoc⟩, x_in_φvoc⟩
-      all_goals subst d_φvoc
-      · refine ⟨φ.voc, Or.inl ?_, x_in_φvoc⟩
-        exact ⟨φ, List.diff_subset R Rcond φ_nocon, rfl⟩
-      all_goals
-        have Rsub := @localRule_does_not_increase_vocab_R _ _ lrule _ res_in x
-        simp at Rsub
-      · specialize Rsub φ.voc (Or.inl ⟨_, φ_L, rfl⟩) x_in_φvoc
-        rcases Rsub with ⟨ψvoc, h_ψvoc, x_in_ψvoc⟩
-        refine ⟨ψvoc, ?_, x_in_ψvoc⟩
-        rcases h_ψvoc with (⟨ψ, ψ_in_Rcond, d_ψvoc⟩ | ⟨ψ, ψ_in_Ocond, d_ψvoc⟩) <;> subst d_ψvoc
-        · exact Or.inl ⟨ψ, preconditionProof.2.1.subset ψ_in_Rcond, rfl⟩
-        · refine Or.inr ⟨ψ, ?_, rfl⟩; aesop
-      · -- whether to use φ.voc depends on whether the localRuleApp changes the O here.
-        rcases O with _|χ <;> rcases Ocond with _|cχ <;> rcases Ores with _|resχ
-        all_goals
-          simp [Olf.change] at * -- already treats 3 cases
-        · specialize Rsub φ.voc (Or.inr ⟨φ, φ_O, rfl⟩) x_in_φvoc
-          rcases Rsub with ⟨ψ, ψ_in_Rcond, x_in_φvoc⟩
-          exact ⟨ψ, preconditionProof.2.subset ψ_in_Rcond, x_in_φvoc⟩
-        · rcases χ with ⟨⟨χ⟩⟩|⟨χ⟩ <;> simp [Olf.R] at *
-          subst φ_O
-          aesop
-        · rcases resχ with ⟨⟨resχ⟩⟩|⟨⟨resχ⟩⟩ <;> simp [Olf.R] at φ_O Rsub
-          subst φ_O
-          simp at x_in_φvoc
-          specialize Rsub (resχ.unload).voc (Or.inr rfl) x_in_φvoc
-          rcases Rsub with ⟨ψ, ψ_in_Rcond, x_in_φvoc⟩
-          exact ⟨ψ.voc, Or.inl ⟨ψ, preconditionProof.2.subset ψ_in_Rcond, rfl⟩, x_in_φvoc⟩
-        · rcases preconditionProof with ⟨Lin, Rin, same_form⟩
-          subst same_form
-          simp at φ_O
-        · specialize Rsub φ.voc (Or.inr ⟨φ, φ_O, rfl⟩) x_in_φvoc
-          rcases Rsub with ⟨ψvoc, ψ_defs, x_in_ψvoc⟩
-          rcases ψ_defs with ⟨ψ, ψ_in, ψvoc_def⟩|⟨ψ, ψ_in, ψvoc_def⟩ <;> subst ψvoc_def
-          · refine ⟨ψ.voc, Or.inl ⟨ψ, preconditionProof.2.1.subset ψ_in, rfl⟩, x_in_ψvoc⟩
-          · refine ⟨ψ.voc, Or.inr ⟨ψ, ?_, rfl⟩, x_in_ψvoc⟩
-            simp_all
-
-/-- Maehara's method for single-step *local* rule applications.
-This covers easy cases without any loaded path repeats.
-We do *not* use `localRuleTruth` to prove this,
-but the more specific lemmas `oneSidedL_sat_down` and `oneSidedL_sat_down`. -/
-def localInterpolantStep (lra : LocalRuleApp)
-    (subθs : ∀ c ∈ lra.C, PartInterpolant c)
-    : PartInterpolant lra.X := by
-  -- UNPACKING TERMS
-  rcases lra with ⟨L, R, o, Lcond, Rcond, Ocond, ress, rule, C, hC, precondProof⟩
-  -- DISTINCTION ON LOCALRULE USED
-  cases def_rule : rule
-  case oneSidedL ress orule YS_def => -- rule applied in first component L
-    let interList := C.attach.map <| fun c => (subθs c.1 c.2).1
-    refine ⟨dis interList, ?_, ?_, ?_⟩ -- disjunction here
-    · intro n n_in_inter
-      rw [in_voc_dis] at n_in_inter
-      rcases n_in_inter with ⟨φ, φ_in, n_in_voc_φ⟩
-      simp only [List.mem_map, List.mem_attach, true_and, Subtype.exists, interList] at φ_in
-      rcases φ_in with ⟨Y, Y_in, def_φ⟩
-      apply localRuleApp_does_not_increase_jvoc _ Y Y_in
-      subst def_φ
-      exact (subθs Y Y_in).prop.1 n_in_voc_φ
-    · rintro nInter_L_sat
-      have LI_sat : satisfiable (Sequent.left (L, R, o) ∪ (interList.map Formula.neg)) := by
-        rcases nInter_L_sat with ⟨W, M, w, w_nInter_L⟩
-        use W, M, w
-        simp only [Sequent.left, Sequent.L, Sequent.O, List.mem_cons, List.mem_append,
-          forall_eq_or_imp, evaluate, disEval, not_exists, not_and] at w_nInter_L
-        simp only [Sequent.left, Sequent.L, Sequent.O, List.mem_union_iff, List.mem_append,
-          List.mem_map]
-        rintro φ (φ_in | ⟨θi,θi_in, φ_def⟩)
-        · apply w_nInter_L.2; assumption
-        · subst φ_def; apply w_nInter_L.1; assumption
-      have := oneSidedL_sat_down ⟨L,R,o⟩ precondProof.1.subset orule YS_def LI_sat
-      rcases this with ⟨⟨L', R', o'⟩, c_in, W, M, w, w_⟩
-      refine (subθs ⟨L', R', o'⟩ (hC ▸ def_rule ▸ c_in)).2.2.1 ⟨W, M, w, ?_⟩ -- given IP property
-      intro φ φ_in; simp at φ_in
-      apply w_; simp [interList]; grind
-    · rintro ⟨W, M, w, w_⟩
-      simp only [Sequent.right, Sequent.R, Sequent.O, List.mem_cons, List.mem_append,
-        forall_eq_or_imp, disEval, List.mem_map, List.mem_attach, true_and, Subtype.exists,
-        interList] at w_
-      rcases w_ with ⟨⟨θi, ⟨c, c_in, def_θi⟩, w_θi⟩, w_R⟩
-      refine (subθs c (hC ▸ c_in)).2.2.2 ⟨W, M, w, ?_⟩ -- given IP property
-      have same_R : c.right = Sequent.right (L,R,o) :=
-        @oneSidedL_preserves_right (L,R,o) _ precondProof.1.subset _ orule _ YS_def c (hC ▸ c_in)
-      rw [same_R]; simp; grind
-  case oneSidedR ress orule YS_def => -- rule applied in second component R
-    -- Only somewhat analogous to oneSidedR. Part 2 and 3 are flipped around in a way.
-    let interList := C.attach.map <| fun c => (subθs c.1 c.2).1
-    refine ⟨Con interList, ?_, ?_, ?_⟩ -- using conjunction here
-    · intro n n_in_inter
-      rw [in_voc_con] at n_in_inter
-      rcases n_in_inter with ⟨φ, φ_in, n_in_voc_φ⟩
-      simp only [List.mem_map, List.mem_attach, true_and, Subtype.exists, interList] at φ_in
-      rcases φ_in with ⟨Y, Y_in, def_φ⟩
-      apply localRuleApp_does_not_increase_jvoc _ Y Y_in
-      subst def_φ
-      exact (subθs Y Y_in).prop.1 n_in_voc_φ
-    · rintro ⟨W, M, w, w_⟩
-      simp only [Sequent.left, Sequent.L, Sequent.O, List.mem_cons, List.mem_append,
-        forall_eq_or_imp, evaluate, conEval, not_forall] at w_
-      rcases w_ with ⟨⟨θi, θi_in, w_nθi⟩, w_L⟩
-      simp only [List.mem_map, List.mem_attach, true_and, Subtype.exists, interList] at θi_in
-      rcases θi_in with ⟨⟨L', R', o'⟩, c_in, def_θi⟩
-      have same_L : Sequent.left ⟨L', R', o'⟩ = Sequent.left (L,R,o) :=
-        @oneSidedR_preserves_left (L,R,o) _ precondProof.2.1.subset _ orule _ YS_def _ (hC ▸ c_in)
-      refine (subθs ⟨L', R', o'⟩ (hC ▸ c_in)).2.2.1 ⟨W, M, w, ?_⟩
-      rw [same_L]; simp; grind
-    · rintro inter_R_sat
-      have RI_sat : satisfiable (Sequent.right (L, R, o) ∪ (interList)) := by
-        rcases inter_R_sat with ⟨W, M, w, w_Inter_R⟩
-        use W, M, w; simp [conEval] at *; grind
-      have := oneSidedR_sat_down ⟨L,R,o⟩ precondProof.2.1.subset orule YS_def RI_sat
-      rcases this with ⟨⟨L', R', o'⟩, c_in, W, M, w, w_⟩
-      refine (subθs ⟨L', R', o'⟩ (hC ▸ def_rule ▸ c_in)).2.2.2 ⟨W, M, w, ?_⟩ -- given IP property
-      intro φ φ_in; simp at φ_in
-      simp [interList, Sequent.right] at w_
-      grind
-  case LRnegL φ =>
-    use φ
-    simp only at subθs
-    simp only [LocalRuleApp.X]
-    refine ⟨?_, ?_, ?_⟩
-    · intro n n_in_φ
-      aesop
-    · rintro ⟨W, M, w, w_⟩
-      simp only [List.empty_eq, List.mem_cons, forall_eq_or_imp, evaluate] at *
-      subst_eqs
-      absurd w_.1
-      have := w_.2 φ
-      simp_all
-    · rintro ⟨W, M, w, w_⟩
-      simp only [List.empty_eq, List.mem_cons, forall_eq_or_imp] at *
-      subst_eqs
-      absurd w_.1
-      have := w_.2 (~φ)
-      simp_all [evaluate]
-  case LRnegR φ =>
-    use ~φ
-    simp only at subθs
-    simp only [LocalRuleApp.X]
-    refine ⟨?_, ?_, ?_⟩
-    · intro n n_in_φ
-      aesop
-    · rintro ⟨W, M, w, w_⟩
-      simp only [List.empty_eq, List.mem_cons, forall_eq_or_imp, evaluate] at *
-      subst_eqs
-      absurd w_.1
-      have := w_.2 (~φ)
-      simp_all [evaluate]
-    · rintro ⟨W, M, w, w_⟩
-      simp only [List.empty_eq, List.mem_cons, forall_eq_or_imp, evaluate] at *
-      subst_eqs
-      absurd w_.1
-      have := w_.2 φ
-      simp_all
-  case loadedL ress χ lrule YS_def =>
-    -- similar to oneSidedL case
-    simp at YS_def
-    let interList := C.attach.map <| fun c => (subθs c.1 c.2).1
-    have O_is_some : Sequent.O (L, R, o) = some (Sum.inl (~'χ)) := by
-        have := precondProof.2.2; simp at this; simp; exact this.symm
-    refine ⟨dis interList, ?_, ?_, ?_⟩ -- disjunction here
-    · intro n n_in_inter
-      rw [in_voc_dis] at n_in_inter
-      rcases n_in_inter with ⟨φ, φ_in, n_in_voc_φ⟩
-      simp only [List.mem_map, List.mem_attach, true_and, Subtype.exists, interList] at φ_in
-      rcases φ_in with ⟨Y, Y_in, def_φ⟩
-      apply localRuleApp_does_not_increase_jvoc _ Y Y_in
-      subst def_φ
-      exact (subθs Y Y_in).prop.1 n_in_voc_φ
-    · rintro nInter_L_sat
-      have LI_sat : satisfiable (Sequent.left (L, R, o) ∪ (interList.map Formula.neg)) := by
-        rcases nInter_L_sat with ⟨W, M, w, w_nInter_L⟩
-        use W, M, w
-        simp only [Sequent.left, Sequent.L, Sequent.O, List.mem_cons, List.mem_append,
-          forall_eq_or_imp, evaluate, disEval, not_exists, not_and] at w_nInter_L
-        simp only [Sequent.left, Sequent.L, Sequent.O, List.mem_union_iff, List.mem_append,
-          List.mem_map]
-        rintro φ (φ_in | ⟨θi,θi_in, φ_def⟩)
-        · apply w_nInter_L.2; assumption
-        · subst φ_def; apply w_nInter_L.1; assumption
-      have := loadedL_sat_down ⟨L,R,o⟩ χ O_is_some lrule YS_def LI_sat
-      rcases this with ⟨⟨L', R', o'⟩, c_in, W, M, w, w_⟩
-      refine (subθs ⟨L', R', o'⟩ (hC ▸ def_rule ▸ c_in)).2.2.1 ⟨W, M, w, ?_⟩ -- given IP property
-      intro φ φ_in; simp at φ_in
-      apply w_; simp [interList]; grind
-    · rintro ⟨W, M, w, w_⟩
-      simp only [Sequent.right, Sequent.R, Sequent.O, List.mem_cons, List.mem_append,
-        forall_eq_or_imp, disEval, List.mem_map, List.mem_attach, true_and, Subtype.exists,
-        interList] at w_
-      rcases w_ with ⟨⟨θi, ⟨c, c_in, def_θi⟩, w_θi⟩, w_R⟩
-      refine (subθs c (hC ▸ c_in)).2.2.2 ⟨W, M, w, ?_⟩ -- given IP property
-      have same_R : c.right = Sequent.right (L,R,o) :=
-        @loadedL_preserves_right ⟨L,R,o⟩ χ O_is_some ress lrule _ YS_def c (hC ▸ c_in)
-      rw [same_R]; simp; grind
-  case loadedR ress χ lrule YS_def =>
-    -- based on oneSidedR case
-    let interList := C.attach.map <| fun c => (subθs c.1 c.2).1
-    have O_is_some : Sequent.O (L, R, o) = some (Sum.inr (~'χ)) := by
-      have := precondProof.2.2; simp at this; simp; exact this.symm
-    refine ⟨Con interList, ?_, ?_, ?_⟩ -- using conjunction here
-    · intro n n_in_inter
-      rw [in_voc_con] at n_in_inter
-      rcases n_in_inter with ⟨φ, φ_in, n_in_voc_φ⟩
-      simp only [List.mem_map, List.mem_attach, true_and, Subtype.exists, interList] at φ_in
-      rcases φ_in with ⟨Y, Y_in, def_φ⟩
-      apply localRuleApp_does_not_increase_jvoc _ Y Y_in
-      subst def_φ
-      exact (subθs Y Y_in).prop.1 n_in_voc_φ
-    · rintro ⟨W, M, w, w_⟩
-      simp only [Sequent.left, Sequent.L, Sequent.O, List.mem_cons, List.mem_append,
-        forall_eq_or_imp, evaluate, conEval, not_forall] at w_
-      rcases w_ with ⟨⟨θi, θi_in, w_nθi⟩, w_L⟩
-      simp only [List.mem_map, List.mem_attach, true_and, Subtype.exists, interList] at θi_in
-      rcases θi_in with ⟨⟨L', R', o'⟩, c_in, def_θi⟩
-      have same_L : Sequent.left ⟨L', R', o'⟩ = Sequent.left (L,R,o) :=
-        @loadedR_preserves_left (L,R,o) _ O_is_some _ lrule _ YS_def _ (hC ▸ c_in)
-      refine (subθs ⟨L', R', o'⟩ (hC ▸ c_in)).2.2.1 ⟨W, M, w, ?_⟩
-      rw [same_L]; simp; grind
-    · rintro inter_R_sat
-      have RI_sat : satisfiable (Sequent.right (L, R, o) ∪ (interList)) := by
-        rcases inter_R_sat with ⟨W, M, w, w_Inter_R⟩
-        use W, M, w; simp [conEval] at *; grind
-      have := loadedR_sat_down ⟨L,R,o⟩ χ O_is_some lrule YS_def RI_sat
-      rcases this with ⟨⟨L', R', o'⟩, c_in, W, M, w, w_⟩
-      refine (subθs ⟨L', R', o'⟩ (hC ▸ def_rule ▸ c_in)).2.2.2 ⟨W, M, w, ?_⟩ -- given IP property
-      intro φ φ_in; simp at φ_in
-      simp only [Sequent.right, Sequent.R_eq, Sequent.O_eq, List.mem_union_iff, List.mem_append,
-        List.mem_map, List.mem_attach, true_and, Subtype.exists, interList] at w_
-      grind
-
-/-! ## Interpolants for Local Tableau -/
-
-def LocalTableau.interpolant (ltX : LocalTableau X)
-    (endθs : ∀ Y ∈ endNodesOf ltX, PartInterpolant Y)
-    : PartInterpolant X := by
-  cases ltX
-  case byLocalRule lra nexts X_def =>
-    subst X_def
-    apply localInterpolantStep lra
-    intro Y Y_in
-    have IH := LocalTableau.interpolant (nexts Y Y_in)
-    exact IH (fun Z Z_in_end => endθs _ (endNodeOfChild_to_endNode lra nexts rfl Y_in Z_in_end))
-  case sim Xbas =>
-    apply endθs X
-    simp [endNodesOf]
 
 /-! ## Interpolants for PdlRules applied to free nodes
 
@@ -561,20 +108,20 @@ lemma clusterListOf_spec (p : PathIn tab) :
   sorry
 
 -- TODO: how to convert `clusterListOf` result back to a tree?
--- Essentially, this would incorporate Lemma 7.22 (a).
+-- Essentially, this would incorporate Lemma 8.14 (a).
 
 def rootOf : List (PathIn tab) → PathIn tab := sorry -- just take the shortest?
 
 -- Or would it be better to already construct (partial) trees instead of lists directly?
 
--- OR just assume are given the root of a cluster and use the tableau as it is to define `Q`?
+-- OR just assume we are given the root of a cluster and use the tableau as it is to define `Q`?
 
-/-- Lemma 7.22 (b) for left side -/
+/-- Lemma 8.14 (b) for left side -/
 lemma cluster_all_left_loaded {p : PathIn tab} (h : (nodeAt p).2.2.isLeft) :
     ∀ q ∈ clusterListOf p, (nodeAt q).2.2.isLeft := by
   sorry
 
-/-- Lemma 7.22 (b) for right side -/
+/-- Lemma 8.14 (b) for right side -/
 lemma cluster_all_right_loaded {p : PathIn tab} (h : (nodeAt p).2.2.isRight) :
     ∀ q ∈ clusterListOf p, (nodeAt q).2.2.isRight := by
   sorry
@@ -585,7 +132,7 @@ instance : Decidable (isExitIn X C) := sorry
 
 /-! ## Quasi-Tableaux -/
 
--- Alternative idea for def 7.31:
+-- Alternative idea for Definition 9.8 quasi-tableau:
 -- Instead of labelling nodes in Q with finite sequents, label them with the path to where
 -- that sequent comes from in `Λ₂[C⁺]`?
 
@@ -602,8 +149,8 @@ open QuasiTab
 
 def Qchildren (C : List Sequent) : (k : Typ) → (Hist : List Sequent) → (X : Sequent) → List QuasiTab
 | .one, Hist, X => -- case k(x)=1
-    if X ∈ Hist ∨ isExitIn X C
-      then [ ] -- then x is a leaf
+    if X ∈ Hist ∨ isExitIn X C -- if x is a repeat (TODO??: in Q) or it is an exit,
+      then [ ] -- then x is a leaf.
       else [ QNode .two X (Qchildren C .two (X :: Hist) X) ]
 | .two, Hist, X => -- case k(x)=2
     [ QNode .three X (Qchildren C .three (X :: Hist) X) ]
@@ -622,7 +169,7 @@ decreasing_by
   · sorry
   · sorry
 
-/-- Quasi-Tableau from Def 7.31. Here we "start the construction", then use `Qchildren`.
+/-- Quasi-Tableau from Def 9.8. Here we "start the construction", then use `Qchildren`.
 No names for the nodes as we use an inductive type, so we just write `X` for `Δₓ` -/
 def Q {r : PathIn tab} : QuasiTab :=
   let X := nodeAt r -- FIXME wlog we only want the right sequent. But `.R` is not enogh !?!?!?!?!?
@@ -874,6 +421,9 @@ lemma IsPartInterpolant.flip : isPartInterpolant X θ → isPartInterpolant X.fl
     simp_all
   · simp_all
   · simp_all
+
+
+/-! ### Cluster Interpolation -/
 
 /-- Given a tableau where the root is loaded, and exit interpolants, interpolate the root. -/
 def clusterInterpolation {Hist L R snlf}
